src/Proof.v
@@ -18,6 +18,31 @@ From Coq Require Import List.
 Require Import Clauses.
 Import ListNotations.
 
+Definition entails cs c :=
+  forall m, ClauseSet.eval m cs = true -> Clause.eval m c = true.
+
+Lemma mem_entails :
+  forall cs c, ClauseSet.mem cs c = true -> entails cs c.
+Proof.
+  intros cs c Hmem m Hm.
+  firstorder using ClauseSet.eval_true_forall.
+Qed.
+
+Lemma resolution :
+  forall (cs : ClauseSet.t) (c1 c2 : Clause.t) (l1 l2 : Literal.t),
+    entails cs (l1::c1) ->
+    entails cs (l2::c2) ->
+    Literal.neg l1 = l2 ->
+    entails cs (c1 ++ c2).
+Proof.
+  intros cs c1 c2 l1 l2 H1 H2 Heq m Hm.
+  specialize (H1 _ Hm); specialize (H2 _ Hm).
+  destruct l1, l2; simpl in *; try easy.
+  all: replace n0 with n in * by congruence.
+  all: destruct (Model.satisfy m n) eqn:E; simpl in *.
+  all: rewrite Clause.eval_app; intuition.
+Qed.
+
 Inductive resolvent : ClauseSet.t -> Clause.t -> Prop :=
   | resolvent_mem : forall cs c,
     ClauseSet.mem cs c = true -> resolvent cs c
@@ -36,86 +61,38 @@ Theorem clause_set_clause_true :
 Proof.
   intros m cs c Hmem Heval.
   firstorder using ClauseSet.eval_true_forall.
-Qed.  
+Qed.
 
 Theorem resolvent_sound :
-  forall m cs c,
+  forall cs c,
     resolvent cs c ->
-    ClauseSet.eval m cs = true ->
-    Clause.eval m c = true.
+    entails cs c.
 Proof.
-  intros m cs c Hres Heval.
-  induction Hres.
-  + apply (ClauseSet.eval_true_forall cs m Heval c H).
-  + pose proof (Hl1 := ClauseSet.eval_true_forall cs m Heval (l1 :: c1) H).
-    pose proof (Hl2 := ClauseSet.eval_true_forall cs m Heval (l2 :: c2) H0).
-    simpl in Hl1, Hl2.
-    destruct (Literal.eval m l1) eqn:E1, (Literal.eval m l2) eqn:E2.
-    * destruct l1, l2; simpl in H1; try discriminate.
-      - inversion H1; subst.
-        simpl in E1, E2.
-        now destruct (Model.satisfy m n0).
-      - inversion H1; subst.
-        simpl in E1, E2.
-        now destruct (Model.satisfy m n0).
-    * apply Clause.eval_true_exists in Hl2 as [x [Hx Hx']].
-      apply Clause.exists_eval_true.
-      exists x; split; auto.
-      apply in_or_app; auto.
-    * apply Clause.eval_true_exists in Hl1 as [x [Hx Hx']].
-      apply Clause.exists_eval_true.
-      exists x; split; auto.
-      apply in_or_app; auto.
-    * destruct l1, l2; simpl in H1; try discriminate.
-      - inversion H1; subst.
-        simpl in E1, E2.
-        now destruct (Model.satisfy m n0).
-      - inversion H1; subst.
-        simpl in E1, E2.
-        now destruct (Model.satisfy m n0).
+  intros cs c Hres.
+  induction Hres as [ cs c Hmem | cs c1 c2 l1 l2 H1%mem_entails H2%mem_entails].
+  + firstorder using ClauseSet.eval_true_forall.
+  + eauto using resolution.
 Qed.
 
 Theorem resolvent_bot_unsat :
   forall cs, resolvent cs [] -> ClauseSet.unsat cs.
 Proof.
   intros cs Hres [m Hm].
-  now pose proof (resolvent_sound m cs _ Hres Hm).
-Qed.
-
-Inductive resolvent_seq : ClauseSet.t -> Clause.t -> Prop :=
-  | resolvent_seq_base : forall cs c,
-    resolvent cs c -> resolvent_seq cs c
-  | resolvent_seq_step : forall cs c c',
-    resolvent cs c ->
-    resolvent_seq (c::cs) c' ->
-    resolvent_seq cs c'.
-
-Lemma resolvent_seq_sound :
-  forall cs c m,
-    resolvent_seq cs c ->
-    ClauseSet.eval m cs = true ->
-    Clause.eval m c = true.
-Proof.
-  intros cs c m Hres Heval.
-  induction Hres.
-  + eauto using resolvent_sound.
-  + eapply IHHres.
-    simpl; apply Bool.andb_true_iff; split; auto.
-    eauto using resolvent_sound.
+  now pose proof (resolvent_sound cs [] Hres _ Hm).
 Qed.
 
 Inductive proof_step : Type :=
   | proof_mem (c : Clause.t)
   | proof_cut (n : nat) (c1 c2 : Clause.t).
 
-Definition conclusion (ut : proof_step) : Clause.t :=
-  match ut with
+Definition conclusion (ps : proof_step) : Clause.t :=
+  match ps with
   | proof_mem c => c
   | proof_cut _ c1 c2 => c1 ++ c2
   end.
 
-Definition is_proof_step (context : ClauseSet.t) (ut : proof_step) : bool :=
-  match ut with
+Definition is_proof_step (context : ClauseSet.t) (ps : proof_step) : bool :=
+  match ps with
   | proof_mem c =>
     ClauseSet.mem context c
   | proof_cut l c1 c2 =>
@@ -124,62 +101,48 @@ Definition is_proof_step (context : ClauseSet.t) (ut : proof_step) : bool :=
   end.
 
 Lemma is_proof_step_sound' :
-  forall ctx ut,
-    is_proof_step ctx ut = true ->
-    resolvent ctx (conclusion ut).
+  forall ctx ps,
+    is_proof_step ctx ps = true ->
+    resolvent ctx (conclusion ps).
 Proof.
-  intros ctx ut.
-  induction ut as [ | l c1 c2 ].
+  intros ctx ps.
+  induction ps as [ | l c1 c2 ].
   - eauto using resolvent.
   - intros [H1 H2]%Bool.andb_true_iff.
     eauto using resolvent.
 Qed.
 
 Lemma is_proof_step_sound :
-  forall ctx ut m,
-    is_proof_step ctx ut = true ->
-    ClauseSet.eval m ctx = true ->
-    Clause.eval m (conclusion ut) = true.
+  forall ctx ps,
+    is_proof_step ctx ps = true ->
+    entails ctx (conclusion ps).
 Proof.
   eauto using resolvent_sound, is_proof_step_sound'.
 Qed.
 
-Fixpoint is_proof (context : ClauseSet.t) (uts : list proof_step) (c : Clause.t) : bool :=
-  match uts with
+Fixpoint is_proof (context : ClauseSet.t) (proof : list proof_step) (c : Clause.t) : bool :=
+  match proof with
   | [] => ClauseSet.mem context c
-  | ut::uts =>
-    is_proof_step context ut &&
-    is_proof ((conclusion ut)::context) uts c
+  | ps::proof =>
+    is_proof_step context ps &&
+    is_proof ((conclusion ps)::context) proof c
   end.
 
-Lemma is_proof_sound' :
-  forall uts ctx c,
-  is_proof ctx uts c = true ->
-  resolvent_seq ctx c.
-Proof.
-  intros uts.
-  induction uts.
-  - eauto using resolvent_seq_base, resolvent_mem.
-  - intros. simpl in H.
-    rewrite Bool.andb_true_iff in H.
-    destruct H as [H1 H2].
-    eapply resolvent_seq_step.
-    + apply (is_proof_step_sound' _ _ H1).
-    + apply (IHuts _ _ H2).
-Qed.
-
 Lemma is_proof_sound :
-  forall uts ctx c m,
-    is_proof ctx uts c = true ->
-    ClauseSet.eval m ctx = true ->
-    Clause.eval m c = true.
+  forall proof ctx c,
+  is_proof ctx proof c = true ->
+  entails ctx c.
 Proof.
-  eauto using resolvent_seq_sound, is_proof_sound'.
+  intros proof. induction proof; simpl.
+  + eauto using mem_entails.
+  + intros ctx c [H1%is_proof_step_sound H2%IHproof]%Bool.andb_true_iff m Hm.
+    specialize (H1 m Hm); specialize (H2 m); simpl in *.
+    intuition.
 Qed.
 
-Theorem resolvent_seq_bot_unsat :
-  forall cs, resolvent_seq cs [] -> ClauseSet.unsat cs.
+Theorem proof_unsat :
+  forall ctx proof, is_proof ctx proof [] = true -> ClauseSet.unsat ctx.
 Proof.
-  intros cs Hres [m Hm].
-  now pose proof (resolvent_seq_sound cs _ m Hres Hm).
+  intros ctx proof Hproof [m Hm].
+  now pose proof (is_proof_sound _ _ _ Hproof _ Hm).
 Qed.
