src/Model.v
@@ -1,0 +1,6 @@
+Class FModel := {
+  eval : nat -> bool
+}.
+
+Coercion eval : FModel >-> Funclass.
+
